Added back forth proofs

Rules.v
@@ -24,8 +24,25 @@ Proof.
   reflexivity.
 Qed.
 
-Theorem inverse_Z_Spider : forall nIn nOut α, ZX_semantics (Z_Spider nIn nOut α) = (ZX_semantics (Z_Spider nIn nOut α))†.
-Abort.
+Theorem trivial_cap_cup : ZX_semantics (Compose Cap Cup) = C2 .* ZX_semantics Empty.
+Proof. simpl; solve_matrix. Qed.
+
+Definition back_forth : ZX 1 1 := Compose (Stack Wire Cap) (Stack Cup Wire).
+
+Theorem back_forth_is_wire : ZX_semantics back_forth = ZX_semantics Wire.
+Proof. 
+  simpl. 
+  rewrite wire_identity_semantics.
+  solve_matrix.
+Qed.
+
+Definition forth_back : ZX 1 1 := Compose (Stack Cap Wire) (Stack Wire Cup).
+Theorem forth_back_is_wire : ZX_semantics back_forth = ZX_semantics Wire.
+Proof.
+  simpl. 
+  rewrite wire_identity_semantics.
+  solve_matrix.
+Qed.
 
 Theorem Z_to_X_with_H_Outputs : forall n m α, ZX_semantics (@Z_Spider n (m * 1) α) = ZX_semantics (Compose (@X_Spider n (m * 1) α) (nStack ZX_H m)).
 Proof.
